@prefix : <http://www.semanticweb.org/medieval-renaissance-manuscripts#> .
@prefix owl: <http://www.w3.org/2002/07/owl#> .
@prefix rdf: <http://www.w3.org/1999/02/22-rdf-syntax-ns#> .
@prefix xml: <http://www.w3.org/XML/1998/namespace> .
@prefix xsd: <http://www.w3.org/2001/XMLSchema#> .
@prefix rdfs: <http://www.w3.org/2000/01/rdf-schema#> .
@base <http://www.semanticweb.org/medieval-renaissance-manuscripts> .

<http://www.semanticweb.org/medieval-renaissance-manuscripts> rdf:type owl:Ontology .

#################################################################
#    Object Properties
#################################################################

###  http://www.semanticweb.org/medieval-renaissance-manuscripts#boughtBook
:boughtBook rdf:type owl:ObjectProperty ;
            owl:inverseOf :sellBook ;
            rdfs:domain :Bookshop ;
            rdfs:range :Publisher ;
            rdfs:comment "sell Book For relates a bookshop with a publisher which publish books thorough it"@en ;
            rdfs:label "sell Book For"@en .


###  http://www.semanticweb.org/medieval-renaissance-manuscripts#hasBookPublisher
:hasBookPublisher rdf:type owl:ObjectProperty ;
                  owl:inverseOf :isBookPublisher ;
                  rdf:type owl:FunctionalProperty ;
                  rdfs:domain :Book ;
                  rdfs:range :Publisher ;
                  rdfs:comment "has Book Publisher relates the book with the publisher that publish it"@en ;
                  rdfs:label "has Book Publisher"@en .


###  http://www.semanticweb.org/medieval-renaissance-manuscripts#hasLibraryLocatedIn
:hasLibraryLocatedIn rdf:type owl:ObjectProperty ;
                     owl:inverseOf :isLibraryLocatedIn ;
                     rdf:type owl:InverseFunctionalProperty ;
                     rdfs:domain :Place ;
                     rdfs:range :Library ;
                     rdfs:comment "has Library Located In relates a Place and a Library located in it"@en ;
                     rdfs:label "has Library Located In"@en .


###  http://www.semanticweb.org/medieval-renaissance-manuscripts#hasManuscriptAuthor
:hasManuscriptAuthor rdf:type owl:ObjectProperty ;
                     owl:inverseOf :isManuscriptAuthor ;
                     rdf:type owl:FunctionalProperty ;
                     rdfs:domain :Manuscript ;
                     rdfs:range :Author ;
                     rdfs:comment "has Manuscript Author relates a manuscript with its author"@en ;
                     rdfs:label "has Manuscript Author"@en .


###  http://www.semanticweb.org/medieval-renaissance-manuscripts#hasManuscriptCollectedIn
:hasManuscriptCollectedIn rdf:type owl:ObjectProperty ;
                          owl:inverseOf :isManuscriptCollectedIn ;
                          rdf:type owl:InverseFunctionalProperty ;
                          rdfs:domain :Library ;
                          rdfs:range :Manuscript ;
                          rdfs:comment "has Manuscript Collected In relates a library with a manuscript that is collected in it"@en ;
                          rdfs:label "has Manuscript Collected In"@en .


###  http://www.semanticweb.org/medieval-renaissance-manuscripts#hasManuscriptGenre
:hasManuscriptGenre rdf:type owl:ObjectProperty ;
                    owl:inverseOf :isManuscriptGenre ;
                    rdfs:domain :Manuscript ;
                    rdfs:range :LiteraryGenre ;
                    rdfs:comment "has Manuscript Genre relates the manuscript with one of its genres"@en ;
                    rdfs:label "has Manuscript Genre"@en .


###  http://www.semanticweb.org/medieval-renaissance-manuscripts#hasManuscriptIncludedIn
:hasManuscriptIncludedIn rdf:type owl:ObjectProperty ;
                         owl:inverseOf :isManuscriptIncludedIn ;
                         rdfs:domain :Book ;
                         rdfs:range :Manuscript ;
                         rdfs:comment "has Manuscript Included In relates a book with a manuscript included in it"@en ;
                         rdfs:label "has Manuscript Included In"@en .


###  http://www.semanticweb.org/medieval-renaissance-manuscripts#hasPublicationAgreement
:hasPublicationAgreement rdf:type owl:ObjectProperty ;
                         owl:inverseOf :isPubblicationAgreement ;
                         rdfs:domain :Publisher ;
                         rdfs:range :Library ;
                         owl:propertyChainAxiom ( :isBookPublisher
                                                  :hasManuscriptIncludedIn
                                                  :isManuscriptCollectedIn
                                                ) ;
                         rdfs:comment "has Publication Agreement relates a publisher with a library which contain a manuscript contained in a book that the publisher publish"@en ;
                         rdfs:label "has Publication Agreement"@en .


###  http://www.semanticweb.org/medieval-renaissance-manuscripts#isBookPublisher
:isBookPublisher rdf:type owl:ObjectProperty ,
                          owl:InverseFunctionalProperty ;
                 rdfs:domain :Publisher ;
                 rdfs:range :Book ;
                 rdfs:comment "is Book Publisher relates a publisher with a book it publishes"@en ;
                 rdfs:label "is Book Publisher"@en .


###  http://www.semanticweb.org/medieval-renaissance-manuscripts#isLibraryLocatedIn
:isLibraryLocatedIn rdf:type owl:ObjectProperty ,
                             owl:FunctionalProperty ;
                    rdfs:domain :Library ;
                    rdfs:range :Place ;
                    rdfs:comment "is Library Located In relates a library with the place in which it is located"@en ;
                    rdfs:label "is Library Located In"@en .


###  http://www.semanticweb.org/medieval-renaissance-manuscripts#isManuscriptAuthor
:isManuscriptAuthor rdf:type owl:ObjectProperty ,
                             owl:InverseFunctionalProperty ;
                    rdfs:domain :Author ;
                    rdfs:range :Manuscript ;
                    rdfs:comment "is Manuscript Author relates an author with its manuscript"@en ;
                    rdfs:label "is Manuscript Author"@en .


###  http://www.semanticweb.org/medieval-renaissance-manuscripts#isManuscriptCollectedIn
:isManuscriptCollectedIn rdf:type owl:ObjectProperty ,
                                  owl:FunctionalProperty ;
                         rdfs:domain :Manuscript ;
                         rdfs:range :Library ;
                         rdfs:comment "is Manuscript Collected In relates a manuscript with the library in which is collected"@en ;
                         rdfs:label "is Manuscript Collected In"@en .


###  http://www.semanticweb.org/medieval-renaissance-manuscripts#isManuscriptGenre
:isManuscriptGenre rdf:type owl:ObjectProperty ;
                   rdfs:domain :LiteraryGenre ;
                   rdfs:range :Manuscript ;
                   rdfs:comment "is Manuscript Genre relates a genre with a manuscript"@en ;
                   rdfs:label "is Manuscript Genre"@en .


###  http://www.semanticweb.org/medieval-renaissance-manuscripts#isManuscriptIncludedIn
:isManuscriptIncludedIn rdf:type owl:ObjectProperty ;
                        rdfs:domain :Manuscript ;
                        rdfs:range :Book ;
                        rdfs:comment "is Manuscript Included In relates a manuscript with a book in which it is included"@en ;
                        rdfs:label "is Manuscript Included In"@en .


###  http://www.semanticweb.org/medieval-renaissance-manuscripts#isPubblicationAgreement
:isPubblicationAgreement rdf:type owl:ObjectProperty ;
                         rdfs:domain :Library ;
                         rdfs:range :Publisher ;
                         rdfs:comment "is Publication Agreement relates a library with a publisher which publish a book that include manuscript contained in that library"@en ;
                         rdfs:label "is Publication Agreement"@en .


###  http://www.semanticweb.org/medieval-renaissance-manuscripts#sellBook
:sellBook rdf:type owl:ObjectProperty ;
          rdfs:domain :Publisher ;
          rdfs:range :Bookshop ;
          rdfs:comment "sell Book Through relates a publisher with a bookshop in which the publisher sell its books"@en ;
          rdfs:label "sell Book Through"@en .


#################################################################
#    Data properties
#################################################################

###  http://www.semanticweb.org/medieval-renaissance-manuscripts#hasBookISBN
:hasBookISBN rdf:type owl:DatatypeProperty ;
             rdfs:subPropertyOf :hasCode ;
             rdf:type owl:FunctionalProperty ;
             rdfs:domain :Book ;
             rdfs:range xsd:string ;
             rdfs:comment "has Book ISBN relates a book with its ISBN Code"@en ;
             rdfs:label "has Book ISBN"@en .


###  http://www.semanticweb.org/medieval-renaissance-manuscripts#hasBookTitle
:hasBookTitle rdf:type owl:DatatypeProperty ;
              rdfs:subPropertyOf :hasTitle ;
              rdf:type owl:FunctionalProperty ;
              rdfs:domain :Book ;
              rdfs:range xsd:string ;
              rdfs:comment "has Book Title relates a book with its book"@en ;
              rdfs:label "has Book Title"@en .


###  http://www.semanticweb.org/medieval-renaissance-manuscripts#hasCode
:hasCode rdf:type owl:DatatypeProperty ,
                  owl:FunctionalProperty ;
         rdfs:comment "has Code relates individuals with its code"@en ;
         rdfs:label "has Code"@en .


###  http://www.semanticweb.org/medieval-renaissance-manuscripts#hasManuscriptDate
:hasManuscriptDate rdf:type owl:DatatypeProperty ,
                            owl:FunctionalProperty ;
                   rdfs:domain :Manuscript ;
                   rdfs:range xsd:dateTime ;
                   rdfs:comment "has Manuscript Date relates a manuscript with its creation date"@en ;
                   rdfs:label "has Manuscript Date"@en .


###  http://www.semanticweb.org/medieval-renaissance-manuscripts#hasManuscriptID
:hasManuscriptID rdf:type owl:DatatypeProperty ;
                 rdfs:subPropertyOf :hasCode ;
                 rdf:type owl:FunctionalProperty ;
                 rdfs:domain :Manuscript ;
                 rdfs:range xsd:string ;
                 rdfs:comment "has Manuscript ID relates a manuscript with its ID"@en ;
                 rdfs:label "has Manuscript ID"@en .


###  http://www.semanticweb.org/medieval-renaissance-manuscripts#hasManuscriptTitle
:hasManuscriptTitle rdf:type owl:DatatypeProperty ;
                    rdfs:subPropertyOf :hasTitle ;
                    rdf:type owl:FunctionalProperty ;
                    rdfs:domain :Manuscript ;
                    rdfs:range xsd:string ;
                    rdfs:comment "has Manuscript Title relates a manuscript with its title"@en ;
                    rdfs:label "has Manuscript Title"@en .


###  http://www.semanticweb.org/medieval-renaissance-manuscripts#hasPublisherID
:hasPublisherID rdf:type owl:DatatypeProperty ;
                rdfs:subPropertyOf :hasCode ;
                rdf:type owl:FunctionalProperty ;
                rdfs:domain :Publisher ;
                rdfs:range xsd:positiveInteger ;
                rdfs:comment "has Publisher ID relates a publisher with its ID"@en ;
                rdfs:label "has Publisher ID"@en .


###  http://www.semanticweb.org/medieval-renaissance-manuscripts#hasPublisherName
:hasPublisherName rdf:type owl:DatatypeProperty ,
                           owl:FunctionalProperty ;
                  rdfs:domain :Publisher ;
                  rdfs:range xsd:string ;
                  rdfs:comment "has Publisher Name relates a publisher with its name"@en ;
                  rdfs:label "has Publisher Name"@en .


###  http://www.semanticweb.org/medieval-renaissance-manuscripts#hasTitle
:hasTitle rdf:type owl:DatatypeProperty ,
                   owl:FunctionalProperty ;
          rdfs:comment "has Title relates an individual with its title"@en ;
          rdfs:label "has Title"@en .


#################################################################
#    Classes
#################################################################

###  http://www.semanticweb.org/medieval-renaissance-manuscripts#Author
:Author rdf:type owl:Class ;
        rdfs:comment "The class that rapresent the author of the Manuscripts"@en ;
        rdfs:label "Author"@en .


###  http://www.semanticweb.org/medieval-renaissance-manuscripts#Book
:Book rdf:type owl:Class ;
      rdfs:subClassOf [ rdf:type owl:Restriction ;
                        owl:onProperty :hasBookPublisher ;
                        owl:qualifiedCardinality "1"^^xsd:nonNegativeInteger ;
                        owl:onClass :Publisher
                      ] ,
                      [ rdf:type owl:Restriction ;
                        owl:onProperty :hasBookISBN ;
                        owl:qualifiedCardinality "1"^^xsd:nonNegativeInteger ;
                        owl:onDataRange xsd:string
                      ] ,
                      [ rdf:type owl:Restriction ;
                        owl:onProperty :hasBookTitle ;
                        owl:qualifiedCardinality "1"^^xsd:nonNegativeInteger ;
                        owl:onDataRange xsd:string
                      ] ;
      rdfs:comment "The class that represent the book in which the manuscripts are included, the book will be publisher throught a Publisher. A book has a title and an ISBN code."@en ;
      rdfs:label "Book"@en .


###  http://www.semanticweb.org/medieval-renaissance-manuscripts#Bookshop
:Bookshop rdf:type owl:Class ;
          rdfs:comment "The class that represent the Bookshop, a bookshop is the way a publisher can sell their books."@en ;
          rdfs:label "Bookshop"@en .


###  http://www.semanticweb.org/medieval-renaissance-manuscripts#Library
:Library rdf:type owl:Class ;
         rdfs:subClassOf [ rdf:type owl:Restriction ;
                           owl:onProperty :isLibraryLocatedIn ;
                           owl:qualifiedCardinality "1"^^xsd:nonNegativeInteger ;
                           owl:onClass :Place
                         ] ;
         owl:disjointUnionOf ( :PrivateLibrary
                               :PublicLibrary
                             ) ;
         rdfs:comment "The class that represent Library, a library is the structure in which the manuscripts are stored, a library is located in exactly one Place. A library can be Public or Private."@en ;
         rdfs:label "Library"@en .


###  http://www.semanticweb.org/medieval-renaissance-manuscripts#LiteraryGenre
:LiteraryGenre rdf:type owl:Class ;
               rdfs:comment "The class that represent the Literary Genre, a manuscript can have one or more literary genre."@en ;
               rdfs:label "Literary Genre"@en .


###  http://www.semanticweb.org/medieval-renaissance-manuscripts#Manuscript
:Manuscript rdf:type owl:Class ;
            rdfs:subClassOf [ rdf:type owl:Restriction ;
                              owl:onProperty :hasManuscriptGenre ;
                              owl:minQualifiedCardinality "1"^^xsd:nonNegativeInteger ;
                              owl:onClass :LiteraryGenre
                            ] ,
                            [ rdf:type owl:Restriction ;
                              owl:onProperty :isManuscriptIncludedIn ;
                              owl:minQualifiedCardinality "1"^^xsd:nonNegativeInteger ;
                              owl:onClass :Book
                            ] ,
                            [ rdf:type owl:Restriction ;
                              owl:onProperty :hasManuscriptAuthor ;
                              owl:qualifiedCardinality "1"^^xsd:nonNegativeInteger ;
                              owl:onClass :Author
                            ] ,
                            [ rdf:type owl:Restriction ;
                              owl:onProperty :isManuscriptCollectedIn ;
                              owl:qualifiedCardinality "1"^^xsd:nonNegativeInteger ;
                              owl:onClass :Library
                            ] ,
                            [ rdf:type owl:Restriction ;
                              owl:onProperty :hasManuscriptDate ;
                              owl:qualifiedCardinality "1"^^xsd:nonNegativeInteger ;
                              owl:onDataRange xsd:dateTime
                            ] ,
                            [ rdf:type owl:Restriction ;
                              owl:onProperty :hasManuscriptID ;
                              owl:qualifiedCardinality "1"^^xsd:nonNegativeInteger ;
                              owl:onDataRange xsd:string
                            ] ,
                            [ rdf:type owl:Restriction ;
                              owl:onProperty :hasManuscriptTitle ;
                              owl:qualifiedCardinality "1"^^xsd:nonNegativeInteger ;
                              owl:onDataRange xsd:string
                            ] ;
            owl:disjointUnionOf ( :MedievalManuscript
                                  :RenaissanceManuscript
                                ) ;
            rdfs:comment "The class that represent the Manuscript, a manuscript has a title, an author, an identifier and a date of creation, a manuscript belong to at least one literary genre and is collected in exactly one library, moreover a manuscript can be Medieval manuscript or a Renaissance manuscript."@en ;
            rdfs:label "Manuscript"@en .


###  http://www.semanticweb.org/medieval-renaissance-manuscripts#MedievalManuscript
:MedievalManuscript rdf:type owl:Class ;
                    rdfs:subClassOf :Manuscript ;
                    rdfs:comment "The class that represent the Medieval Manuscript that is a sub-class of Manuscript."@en ;
                    rdfs:label "Medieval Manuscript"@en .


###  http://www.semanticweb.org/medieval-renaissance-manuscripts#Place
:Place rdf:type owl:Class ;
       rdfs:comment "The class that represent the Place, a place is where a library is located."@en ;
       rdfs:label "Place"@en .


###  http://www.semanticweb.org/medieval-renaissance-manuscripts#PrivateLibrary
:PrivateLibrary rdf:type owl:Class ;
                rdfs:subClassOf :Library ;
                rdfs:comment "The class that represent the PrivateLibrary that is a sub-class of Library."@en ;
                rdfs:label "Private Library"@en .


###  http://www.semanticweb.org/medieval-renaissance-manuscripts#PublicLibrary
:PublicLibrary rdf:type owl:Class ;
               rdfs:subClassOf :Library ;
               rdfs:comment "The class that represent the PublicLibrary that is a sub-class of Library."@en ;
               rdfs:label "Public Library"@en .


###  http://www.semanticweb.org/medieval-renaissance-manuscripts#Publisher
:Publisher rdf:type owl:Class ;
           rdfs:subClassOf [ rdf:type owl:Restriction ;
                             owl:onProperty :hasPublicationAgreement ;
                             owl:someValuesFrom :Library
                           ] ,
                           [ rdf:type owl:Restriction ;
                             owl:onProperty :isBookPublisher ;
                             owl:minQualifiedCardinality "2"^^xsd:nonNegativeInteger ;
                             owl:onClass :Book
                           ] ,
                           [ rdf:type owl:Restriction ;
                             owl:onProperty :sellBook ;
                             owl:minQualifiedCardinality "2"^^xsd:nonNegativeInteger ;
                             owl:onClass :Bookshop
                           ] ,
                           [ rdf:type owl:Restriction ;
                             owl:onProperty :hasPublisherID ;
                             owl:qualifiedCardinality "1"^^xsd:nonNegativeInteger ;
                             owl:onDataRange xsd:positiveInteger
                           ] ,
                           [ rdf:type owl:Restriction ;
                             owl:onProperty :hasPublisherName ;
                             owl:qualifiedCardinality "1"^^xsd:nonNegativeInteger ;
                             owl:onDataRange xsd:string
                           ] ;
           rdfs:comment "The class that represent a Publisher. A publisher sells the published books throught  a bookshop, a publisher is identified by a name and an ID, moreover a publisher has a publication agreement with the library in which the manuscripts, inside its published books, are collected."@en ;
           rdfs:label "Publisher"@en .


###  http://www.semanticweb.org/medieval-renaissance-manuscripts#RenaissanceManuscript
:RenaissanceManuscript rdf:type owl:Class ;
                       rdfs:subClassOf :Manuscript ;
                       rdfs:comment "The class that represent the Renaissance Manuscript that is a sub-class of Manuscript."@en ;
                       rdfs:label "Renaissance Manuscript"@en .


#################################################################
#    Individuals
#################################################################

###  http://www.semanticweb.org/medieval-renaissance-manuscripts#ariosto
:ariosto rdf:type owl:NamedIndividual ,
                  :Author .


###  http://www.semanticweb.org/medieval-renaissance-manuscripts#codexRegius
:codexRegius rdf:type owl:NamedIndividual ,
                      :RenaissanceManuscript ;
             :hasManuscriptAuthor :ariosto ;
             :hasManuscriptGenre :genereEpico ;
             :isManuscriptCollectedIn :libreriaLaurenziana ;
             :isManuscriptIncludedIn :tantiRacconti ;
             :hasManuscriptDate "1235-01-01T00:00:00"^^xsd:dateTime ;
             :hasManuscriptID "efgh"^^xsd:string ;
             :hasManuscriptTitle "Codex Regius"^^xsd:string .


###  http://www.semanticweb.org/medieval-renaissance-manuscripts#dante
:dante rdf:type owl:NamedIndividual ,
                :Author .


###  http://www.semanticweb.org/medieval-renaissance-manuscripts#discorsiRinascimentali
:discorsiRinascimentali rdf:type owl:NamedIndividual ,
                                 :Book ;
                        :hasBookPublisher :harperCollins ;
                        :hasBookISBN "ISBN:zzz"^^xsd:string ;
                        :hasBookTitle "Discorsi Rinascimentali"^^xsd:string .


###  http://www.semanticweb.org/medieval-renaissance-manuscripts#fantasieBarocche
:fantasieBarocche rdf:type owl:NamedIndividual ,
                           :Book ;
                  :hasBookPublisher :harperCollins ;
                  :hasBookISBN "ISBN:tyu"^^xsd:string ;
                  :hasBookTitle "Fantasie Barocche"^^xsd:string .


###  http://www.semanticweb.org/medieval-renaissance-manuscripts#feltrinelli
:feltrinelli rdf:type owl:NamedIndividual ,
                      :Bookshop .


###  http://www.semanticweb.org/medieval-renaissance-manuscripts#genereEpico
:genereEpico rdf:type owl:NamedIndividual ,
                      :LiteraryGenre .


###  http://www.semanticweb.org/medieval-renaissance-manuscripts#harperCollins
:harperCollins rdf:type owl:NamedIndividual ,
                        :Publisher ;
               :isBookPublisher :leMiglioriRaccolteMedievali ,
                                :tantiRacconti ;
               :sellBook :feltrinelli ,
                         :mondadori ;
               :hasPublisherID "1234"^^xsd:positiveInteger ;
               :hasPublisherName "Harper Collins"^^xsd:string .


###  http://www.semanticweb.org/medieval-renaissance-manuscripts#leMiglioriRaccolteMedievali
:leMiglioriRaccolteMedievali rdf:type owl:NamedIndividual ,
                                      :Book ;
                             :hasBookPublisher :harperCollins ;
                             :hasBookISBN "ISBN:abcd"^^xsd:string ;
                             :hasBookTitle "Le Migliori Raccolte Medievali"^^xsd:string .


###  http://www.semanticweb.org/medieval-renaissance-manuscripts#libreriaComunale
:libreriaComunale rdf:type owl:NamedIndividual ,
                           :PublicLibrary ;
                  :isLibraryLocatedIn :roma .


###  http://www.semanticweb.org/medieval-renaissance-manuscripts#libreriaLaurenziana
:libreriaLaurenziana rdf:type owl:NamedIndividual ,
                              :PrivateLibrary ;
                     :isLibraryLocatedIn :pisa .


###  http://www.semanticweb.org/medieval-renaissance-manuscripts#libroDiKells
:libroDiKells rdf:type owl:NamedIndividual ,
                       :MedievalManuscript ;
              :hasManuscriptAuthor :dante ;
              :hasManuscriptGenre :genereEpico ;
              :isManuscriptCollectedIn :libreriaComunale ;
              :isManuscriptIncludedIn :leMiglioriRaccolteMedievali ;
              :hasManuscriptDate "1400-01-01T00:00:00"^^xsd:dateTime ;
              :hasManuscriptID "abcd"^^xsd:string ;
              :hasManuscriptTitle "Libro Di Kells"^^xsd:string .


###  http://www.semanticweb.org/medieval-renaissance-manuscripts#mondadori
:mondadori rdf:type owl:NamedIndividual ,
                    :Bookshop .


###  http://www.semanticweb.org/medieval-renaissance-manuscripts#papiriDiErcolano
:papiriDiErcolano rdf:type owl:NamedIndividual ,
                           :MedievalManuscript ;
                  :hasManuscriptAuthor :dante ;
                  :hasManuscriptGenre :genereEpico ;
                  :isManuscriptCollectedIn :libreriaComunale ;
                  :isManuscriptIncludedIn :leMiglioriRaccolteMedievali ;
                  :hasManuscriptDate "1220-01-01T00:00:00"^^xsd:dateTime ;
                  :hasManuscriptID "ijkl"^^xsd:string ;
                  :hasManuscriptTitle "Papiri Di Ercolano"^^xsd:string .


###  http://www.semanticweb.org/medieval-renaissance-manuscripts#pisa
:pisa rdf:type owl:NamedIndividual ,
               :Place .


###  http://www.semanticweb.org/medieval-renaissance-manuscripts#roma
:roma rdf:type owl:NamedIndividual ,
               :Place .


###  http://www.semanticweb.org/medieval-renaissance-manuscripts#storieDellaBuonanotte
:storieDellaBuonanotte rdf:type owl:NamedIndividual ,
                                :Book ;
                       :hasBookPublisher :harperCollins ;
                       :hasBookISBN "ISBN: rrrr"^^xsd:string ;
                       :hasBookTitle "Storie Della Buonanotte"^^xsd:string .


###  http://www.semanticweb.org/medieval-renaissance-manuscripts#tantiRacconti
:tantiRacconti rdf:type owl:NamedIndividual ,
                        :Book ;
               :hasBookPublisher :harperCollins ;
               :hasBookISBN "ISBN:efgh"^^xsd:string ;
               :hasBookTitle "Tanti Racconti"^^xsd:string .


#################################################################
#    General axioms
#################################################################

[ rdf:type owl:AllDisjointClasses ;
  owl:members ( :Author
                :Book
                :Bookshop
                :Library
                :LiteraryGenre
                :Manuscript
                :Place
                :Publisher
              )
] .


###  Generated by the OWL API (version 4.5.9.2019-02-01T07:24:44Z) https://github.com/owlcs/owlapi
